\section*{Properties of Summations}
\begin{align*}
    & \sum_{i=m}^n (k \cdot a_i) = k \sum_{i=m}^n a_i.  \;\;\;\; \sum_{i=1}^n c = n \cdot c. \;\;\;\; \sum_{i=m}^n (a_i \pm b_i) = \sum_{i=m}^n a_i \pm \sum_{i=m}^n b_i.\\
    &\sum_{i=m}^n a_i = \sum_{j=m+k}^{n+k} a_{j-k} \;\;\;\; \sum_{i=m}^n a_i = \sum_{i=m}^p a_i + \sum_{i=p+1}^n a_i \\
    &\sum_{i=m}^n (a_i - a_{i-1}) = a_n - a_{m-1}. \;\;\;\; \sum_{i=1}^n \sum_{j=1}^m a_{ij} = \sum_{j=1}^m \sum_{i=1}^n a_{ij}.
    \\
    &\bullet  \sum_{i=1}^n i = \frac{n(n+1)}{2}.\;\;\;\; \bullet  \sum_{i=1}^n i^2 = \frac{n(n+1)(2n+1)}{6}. \;\;\;\; \bullet  \sum_{i=0}^{n-1} r^i = \frac{1-r^n}{1-r}.
\end{align*}
