\section*{Vector Identities Products}
\begin{align*}
&\mathbf{A} \cdot (\mathbf{B} \times \mathbf{C}) = \mathbf{B} \cdot (\mathbf{C} \times \mathbf{A}) = \mathbf{C} \cdot (\mathbf{A} \times \mathbf{B}) \\
&\mathbf{A} \times (\mathbf{B} \times \mathbf{C}) = \mathbf{B}(\mathbf{A} \cdot \mathbf{C}) - \mathbf{C}(\mathbf{A} \cdot \mathbf{B}) \\
&\nabla(fg) = f\nabla g + g\nabla f \\
&\nabla(\mathbf{A} \cdot \mathbf{B}) = \mathbf{A} \times (\nabla \times \mathbf{B}) + \mathbf{B} \times (\nabla \times \mathbf{A}) + (\mathbf{A} \cdot \nabla)\mathbf{B} + (\mathbf{B} \cdot \nabla)\mathbf{A} \\
&\nabla \cdot (f\mathbf{A}) = f(\nabla \cdot \mathbf{A}) + \mathbf{A} \cdot \nabla f \\
&\nabla \cdot (\mathbf{A} \times \mathbf{B}) = \mathbf{B} \cdot (\nabla \times \mathbf{A}) - \mathbf{A} \cdot (\nabla \times \mathbf{B}) \\
&\nabla \times (f\mathbf{A}) = f(\nabla \times \mathbf{A}) - \mathbf{A} \times \nabla f \\
&\nabla \times (\mathbf{A} \times \mathbf{B}) = (\mathbf{B} \cdot \nabla)\mathbf{A} - (\mathbf{A} \cdot \nabla)\mathbf{B} + \mathbf{A}(\nabla \cdot \mathbf{B}) - \mathbf{B}(\nabla \cdot \mathbf{A}) \\
&\nabla \cdot (\nabla \times \mathbf{A}) = \nabla \times (\nabla f) = 0 \\
&\nabla \times (\nabla \times \mathbf{A}) = \nabla (\nabla \cdot \mathbf{A}) - \nabla^2 \mathbf{A}\\
&\textstyle \int_a^b \nabla f \cdot d\mathbf{r} = f(b){-}f(a) \;\;\;\;
\iiint_V (\nabla{\cdot}\mathbf{F}) dV = \oiint_S \mathbf{F}{\cdot}\hat{\mathbf{n}}\,dS \;\;\;\;
\iint_\Sigma (\nabla{\times}\mathbf{F}){\cdot}d\mathbf{S} = \oint_{\partial\Sigma} \mathbf{F}{\cdot}d\mathbf{r}\\
&\tfrac{d}{dx}\textstyle \int_{h(x)}^{g(x)} f(t) \, dt =  f\big(g(x)\big) \cdot g'(x) - f\big(h(x)\big) \cdot h'(x)
\end{align*}
